Show that Equation (8) implies Equation (5).
\\

\deepersection{Solution}

Note that Equation (8) from Lecture 0 is:

\begin{align}
    V(k) = \underset{c, k'}{\text{max }} u(c) + \beta V(k') 
\end{align}

subject to

\begin{align}
    c + k' \leq f(k) + (1 - \delta)k
\end{align}

Consider the Lagrangian for this equation:

\begin{align}
    \mathcal{L} = u(c) + \beta V(k_+) + \lambda(f(k) + (1-\delta)k - c - k_+)
\end{align}

Now, we take the FOCs:

\begin{align}
    \frac{\partial \mathcal{L}}{\partial c} &= u'(c) - \lambda = 0 \label{eq:pset_2023_24_ps1_q1_golosov_foc1} \\
    \frac{\partial \mathcal{L}}{\partial k_+} &= \beta V'(k_+) - \lambda = 0 \label{eq:pset_2023_24_ps1_q1_golosov_foc2}
\end{align}

The envelope condition\footnote{\href{https://www.sfu.ca/~wainwrig/Econ331/env-theorem2.pdf}{Notes on Envelope Theorem}; \href{https://en.wikipedia.org/wiki/Envelope_theorem}{Wikipedia Page on Envelope Theorem}} is:

\begin{align}
    V'(k) = \frac{\partial \mathcal{L}}{\partial k} = \lambda f'(k) + \lambda(1-\delta) = \lambda[f'(k) + (1 - \delta)]
\end{align}

From \eqref{eq:pset_2023_24_ps1_q1_golosov_foc1} and \eqref{eq:pset_2023_24_ps1_q1_golosov_foc2}, we have:

\begin{align}
    \lambda = u'(c) = \beta V'(k_+) \label{eq:pset_2023_24_ps1_q1_golosov_lambda}
\end{align}

Applying them to one period earlier gives:

\begin{align}
    \lambda = u'(c_-) = \beta V'(k) \label{eq:pset_2023_24_ps1_q1_golosov_lambda_earlier}
\end{align} 

Now, use \eqref{eq:pset_2023_24_ps1_q1_golosov_lambda} and \eqref{eq:pset_2023_24_ps1_q1_golosov_lambda_earlier} to
replace $\lambda$ and $V'(k)$ in the envelope condition:

\begin{align}
    &\frac{u'(c_{-})}{\beta} = u'(c)(f'(k) + (1 - \delta)) \\
    \Leftrightarrow & u'(c_{-}) = \beta u'(c)(f'(k) + (1 - \delta))
\end{align}

By re-arranging terms and moving our time indicators up by 2 periods, this gives:

\begin{align}
    u'(c_t) = \beta[1 + f'(k_{t+1}) - \delta]u'(c_{t+1})
\end{align}

which is Equation (5).